{
"cells": [
{"cell_type":    "code", "execution_count":null, "metadata":{}, "source":["%%html\n<link href=\"http://mathbook.pugetsound.edu/beta/mathbook-content.css\" rel=\"stylesheet\" type=\"text/css\" />\n<link href=\"https://aimath.org/mathbook/mathbook-add-on.css\" rel=\"stylesheet\" type=\"text/css\" />\n<style>.subtitle {font-size:medium; display:block}</style>\n<link href=\"https://fonts.googleapis.com/css?family=Open+Sans:400,400italic,600,600italic\" rel=\"stylesheet\" type=\"text/css\" />\n<link href=\"https://fonts.googleapis.com/css?family=Inconsolata:400,700&subset=latin,latin-ext\" rel=\"stylesheet\" type=\"text/css\" /><!-- Hide this cell. -->\n<script>\nvar cell = $(\".container .cell\").eq(0), ia = cell.find(\".input_area\")\nif (cell.find(\".toggle-button\").length == 0) {\nia.after(\n    $('<button class=\"toggle-button\">Toggle hidden code</button>').click(\n        function (){ ia.toggle() }\n        )\n    )\nia.hide()\n}\n</script>\n"], "outputs":[]},
{"cell_type":"markdown", "metadata":{}, "source":["**Important:** to view this notebook properly you will need to execute the cell above, which assumes you have an Internet connection.  It should already be selected, or place your cursor anywhere above to select.  Then press the \"Run\" button in the menu bar above (the right-pointing arrowhead), or press Shift-Enter on your keyboard."]},
{"cell_type":"markdown", "metadata":{}, "source":["$\\newcommand{\\identity}{\\mathrm{id}}\n\\newcommand{\\notdivide}{\\nmid}\n\\newcommand{\\notsubset}{\\not\\subset}\n\\newcommand{\\lcm}{\\operatorname{lcm}}\n\\newcommand{\\gf}{\\operatorname{GF}}\n\\newcommand{\\inn}{\\operatorname{Inn}}\n\\newcommand{\\aut}{\\operatorname{Aut}}\n\\newcommand{\\Hom}{\\operatorname{Hom}}\n\\newcommand{\\cis}{\\operatorname{cis}}\n\\newcommand{\\chr}{\\operatorname{char}}\n\\newcommand{\\Null}{\\operatorname{Null}}\n\\newcommand{\\lt}{<}\n\\newcommand{\\gt}{>}\n\\newcommand{\\amp}{&}\n$"]},
{"cell_type":"markdown", "metadata":{}, "source":["<div class=\"mathbook-content\"><h2 class=\"heading hide-type\" alt=\"Exercises 1.3 Exercises\"><span class=\"type\">Section</span><span class=\"codenumber\">1.3</span><span class=\"title\">Exercises</span></h2><a href=\"exercises-sets.ipynb\" class=\"permalink\">¶</a></div>"]},
{"cell_type":"markdown", "metadata":{}, "source":["<div class=\"mathbook-content\"><article class=\"exercise-like\" id=\"exercise-1\"><h6 class=\"heading\"><span class=\"codenumber\">1</span></h6><p id=\"p-118\">Suppose that</p><div class=\"displaymath\">\n\\begin{align*}\nA & = \\{ x : x \\in \\mathbb N \\text{ and } x \\text{ is even} \\},\\\\\nB & = \\{x : x \\in \\mathbb N \\text{ and } x \\text{ is prime}\\},\\\\\nC & = \\{ x : x \\in \\mathbb N \\text{ and } x \\text{ is a multiple of 5}\\}.\n\\end{align*}\n</div><p>Describe each of the following sets. </p><ol class=\"lower-alpha cols2\"><li id=\"li-38\"><p id=\"p-119\">$A \\cap B$</p></li><li id=\"li-39\"><p id=\"p-120\">$B \\cap C$</p></li><li id=\"li-40\"><p id=\"p-121\">$A \\cup B$</p></li><li id=\"li-41\"><p id=\"p-122\">$A \\cap (B \\cup C)$</p></li></ol><div class=\"solutions\"><span class=\"solution\"><a knowl=\"\" class=\"id-ref\" refid=\"hk-hint-1\" id=\"hint-1\"><span class=\"type\">Hint</span></a></span><div id=\"hk-hint-1\" class=\"hidden-content tex2jax_ignore\"><span class=\"solution\"><p id=\"p-123\">(a) $A \\cap B = \\{ 2 \\}\\text{;}$ (b) $B \\cap C = \\{ 5 \\}\\text{.}$</p></span></div></div></article></div>"]},
{"cell_type":"markdown", "metadata":{}, "source":["<div class=\"mathbook-content\"><article class=\"exercise-like\" id=\"exercise-2\"><h6 class=\"heading\"><span class=\"codenumber\">2</span></h6><p id=\"p-124\">If $A = \\{ a, b, c \\}\\text{,}$ $B = \\{ 1, 2, 3 \\}\\text{,}$ $C = \\{ x \\}\\text{,}$ and $D = \\emptyset\\text{,}$ list all of the elements in each of the following sets. </p><ol class=\"lower-alpha cols2\"><li id=\"li-42\"><p id=\"p-125\">$A \\times B$</p></li><li id=\"li-43\"><p id=\"p-126\">$B \\times A$</p></li><li id=\"li-44\"><p id=\"p-127\">$A \\times B \\times C$</p></li><li id=\"li-45\"><p id=\"p-128\">$A \\times D$</p></li></ol><div class=\"solutions\"><span class=\"solution\"><a knowl=\"\" class=\"id-ref\" refid=\"hk-hint-2\" id=\"hint-2\"><span class=\"type\">Hint</span></a></span><div id=\"hk-hint-2\" class=\"hidden-content tex2jax_ignore\"><span class=\"solution\"><p id=\"p-129\">(a) $A \\times B = \\{ (a,1), (a,2), (a,3), (b,1), (b,2), (b,3), (c,1), (c,2), (c,3) \\}\\text{;}$ (d) $A \\times D = \\emptyset\\text{.}$</p></span></div></div></article></div>"]},
{"cell_type":"markdown", "metadata":{}, "source":["<div class=\"mathbook-content\"><article class=\"exercise-like\" id=\"exercise-3\"><h6 class=\"heading\"><span class=\"codenumber\">3</span></h6><p id=\"p-130\">Find an example of two nonempty sets $A$ and $B$ for which $A \\times B = B \\times A$ is true.</p></article></div>"]},
{"cell_type":"markdown", "metadata":{}, "source":["<div class=\"mathbook-content\"><article class=\"exercise-like\" id=\"exercise-4\"><h6 class=\"heading\"><span class=\"codenumber\">4</span></h6><p id=\"p-131\">Prove  $A \\cup \\emptyset = A$ and $A \\cap \\emptyset = \\emptyset\\text{.}$</p></article></div>"]},
{"cell_type":"markdown", "metadata":{}, "source":["<div class=\"mathbook-content\"><article class=\"exercise-like\" id=\"exercise-5\"><h6 class=\"heading\"><span class=\"codenumber\">5</span></h6><p id=\"p-132\">Prove $A \\cup B = B \\cup A$ and $A \\cap B = B \\cap A\\text{.}$</p></article></div>"]},
{"cell_type":"markdown", "metadata":{}, "source":["<div class=\"mathbook-content\"><article class=\"exercise-like\" id=\"exercise-6\"><h6 class=\"heading\"><span class=\"codenumber\">6</span></h6><p id=\"p-133\">Prove $A \\cup (B \\cap C) = (A \\cup B) \\cap (A \\cup C)\\text{.}$</p><div class=\"solutions\"><span class=\"solution\"><a knowl=\"\" class=\"id-ref\" refid=\"hk-hint-3\" id=\"hint-3\"><span class=\"type\">Hint</span></a></span><div id=\"hk-hint-3\" class=\"hidden-content tex2jax_ignore\"><span class=\"solution\"><p id=\"p-134\">If $x \\in A \\cup (B \\cap C)\\text{,}$ then either $x \\in A$ or $x \\in B \\cap C\\text{.}$  Thus,   $x \\in A \\cup B$ and $A \\cup C\\text{.}$  Hence, $x \\in (A \\cup B) \\cap (A \\cup C)\\text{.}$ Therefore, $A \\cup (B \\cap C) \\subset (A \\cup B) \\cap (A \\cup C)\\text{.}$  Conversely, if $x \\in (A \\cup B) \\cap (A \\cup C)\\text{,}$ then $x \\in A \\cup B$ and $A \\cup C\\text{.}$ Thus, $x \\in A$ or $x$ is in both $B$ and $C\\text{.}$ So $x \\in A \\cup (B \\cap C)$ and therefore $(A \\cup B) \\cap (A \\cup C) \\subset A \\cup (B \\cap C)\\text{.}$ Hence, $A \\cup (B \\cap C) = (A \\cup B) \\cap (A \\cup C)\\text{.}$</p></span></div></div></article></div>"]},
{"cell_type":"markdown", "metadata":{}, "source":["<div class=\"mathbook-content\"><article class=\"exercise-like\" id=\"exercise-7\"><h6 class=\"heading\"><span class=\"codenumber\">7</span></h6><p id=\"p-135\">Prove $A \\cap (B \\cup C) = (A \\cap B) \\cup (A \\cap C)\\text{.}$</p></article></div>"]},
{"cell_type":"markdown", "metadata":{}, "source":["<div class=\"mathbook-content\"><article class=\"exercise-like\" id=\"exercise-8\"><h6 class=\"heading\"><span class=\"codenumber\">8</span></h6><p id=\"p-136\">Prove  $A \\subset B$ if and only if $A \\cap B = A\\text{.}$</p></article></div>"]},
{"cell_type":"markdown", "metadata":{}, "source":["<div class=\"mathbook-content\"><article class=\"exercise-like\" id=\"exercise-9\"><h6 class=\"heading\"><span class=\"codenumber\">9</span></h6><p id=\"p-137\">Prove $(A \\cap B)' = A' \\cup B'\\text{.}$</p></article></div>"]},
{"cell_type":"markdown", "metadata":{}, "source":["<div class=\"mathbook-content\"><article class=\"exercise-like\" id=\"exercise-10\"><h6 class=\"heading\"><span class=\"codenumber\">10</span></h6><p id=\"p-138\">Prove  $A \\cup B = (A \\cap B) \\cup (A \\setminus B) \\cup (B \\setminus A)\\text{.}$</p><div class=\"solutions\"><span class=\"solution\"><a knowl=\"\" class=\"id-ref\" refid=\"hk-hint-4\" id=\"hint-4\"><span class=\"type\">Hint</span></a></span><div id=\"hk-hint-4\" class=\"hidden-content tex2jax_ignore\"><span class=\"solution\"><p id=\"p-139\">$(A \\cap B) \\cup (A \\setminus B) \\cup (B \\setminus A) = (A \\cap B) \\cup (A \\cap B') \\cup (B \\cap A') = [A \\cap (B \\cup B')] \\cup (B \\cap A') = A \\cup (B \\cap A') = (A \\cup B) \\cap (A \\cup A') = A \\cup B\\text{.}$</p></span></div></div></article></div>"]},
{"cell_type":"markdown", "metadata":{}, "source":["<div class=\"mathbook-content\"><article class=\"exercise-like\" id=\"exercise-11\"><h6 class=\"heading\"><span class=\"codenumber\">11</span></h6><p id=\"p-140\">Prove  $(A \\cup B) \\times C = (A \\times C ) \\cup (B \\times C)\\text{.}$</p></article></div>"]},
{"cell_type":"markdown", "metadata":{}, "source":["<div class=\"mathbook-content\"><article class=\"exercise-like\" id=\"exercise-12\"><h6 class=\"heading\"><span class=\"codenumber\">12</span></h6><p id=\"p-141\">Prove  $(A \\cap B) \\setminus B = \\emptyset\\text{.}$</p></article></div>"]},
{"cell_type":"markdown", "metadata":{}, "source":["<div class=\"mathbook-content\"><article class=\"exercise-like\" id=\"exercise-13\"><h6 class=\"heading\"><span class=\"codenumber\">13</span></h6><p id=\"p-142\">Prove  $(A \\cup B) \\setminus B = A \\setminus B\\text{.}$</p></article></div>"]},
{"cell_type":"markdown", "metadata":{}, "source":["<div class=\"mathbook-content\"><article class=\"exercise-like\" id=\"exercise-14\"><h6 class=\"heading\"><span class=\"codenumber\">14</span></h6><p id=\"p-143\">Prove  $A \\setminus (B \\cup C) = (A \\setminus B) \\cap (A \\setminus C)\\text{.}$</p><div class=\"solutions\"><span class=\"solution\"><a knowl=\"\" class=\"id-ref\" refid=\"hk-hint-5\" id=\"hint-5\"><span class=\"type\">Hint</span></a></span><div id=\"hk-hint-5\" class=\"hidden-content tex2jax_ignore\"><span class=\"solution\"><p id=\"p-144\">$A \\setminus (B \\cup C) = A \\cap (B \\cup C)' = (A \\cap A) \\cap (B' \\cap C') = (A \\cap B') \\cap (A \\cap C') = (A \\setminus B) \\cap (A \\setminus C)\\text{.}$</p></span></div></div></article></div>"]},
{"cell_type":"markdown", "metadata":{}, "source":["<div class=\"mathbook-content\"><article class=\"exercise-like\" id=\"exercise-15\"><h6 class=\"heading\"><span class=\"codenumber\">15</span></h6><p id=\"p-145\">Prove  $A \\cap (B \\setminus C) = (A \\cap B) \\setminus (A \\cap C)\\text{.}$</p></article></div>"]},
{"cell_type":"markdown", "metadata":{}, "source":["<div class=\"mathbook-content\"><article class=\"exercise-like\" id=\"exercise-16\"><h6 class=\"heading\"><span class=\"codenumber\">16</span></h6><p id=\"p-146\">Prove  $(A \\setminus B) \\cup (B \\setminus A) = (A \\cup B) \\setminus (A \\cap B)\\text{.}$</p></article></div>"]},
{"cell_type":"markdown", "metadata":{}, "source":["<div class=\"mathbook-content\"><article class=\"exercise-like\" id=\"exercise-17\"><h6 class=\"heading\"><span class=\"codenumber\">17</span></h6><p id=\"p-147\">Which of the following relations $f: {\\mathbb Q} \\rightarrow {\\mathbb Q}$ define a mapping? In each case, supply a reason why $f$ is or is not a mapping. </p><ol class=\"lower-alpha cols2\"><li id=\"li-46\"><p id=\"p-148\">$\\displaystyle f(p/q) = \\frac{p+ 1}{p - 2}$</p></li><li id=\"li-47\"><p id=\"p-149\">$\\displaystyle f(p/q) = \\frac{3p}{3q}$</p></li><li id=\"li-48\"><p id=\"p-150\">$\\displaystyle f(p/q) = \\frac{p+q}{q^2}$</p></li><li id=\"li-49\"><p id=\"p-151\">$\\displaystyle f(p/q) = \\frac{3 p^2}{7 q^2} - \\frac{p}{q}$</p></li></ol><div class=\"solutions\"><span class=\"solution\"><a knowl=\"\" class=\"id-ref\" refid=\"hk-hint-6\" id=\"hint-6\"><span class=\"type\">Hint</span></a></span><div id=\"hk-hint-6\" class=\"hidden-content tex2jax_ignore\"><span class=\"solution\"><p id=\"p-152\">(a) Not a map since $f(2/3)$ is undefined; (b) this is a map; (c) not a map, since $f(1/2) = 3/4$ but $f(2/4)=3/8\\text{;}$ (d) this is a map.</p></span></div></div></article></div>"]},
{"cell_type":"markdown", "metadata":{}, "source":["<div class=\"mathbook-content\"><article class=\"exercise-like\" id=\"exercise-18\"><h6 class=\"heading\"><span class=\"codenumber\">18</span></h6><p id=\"p-153\">Determine which of the following functions are one-to-one and which are onto.  If the function is not onto, determine its range. </p><ol class=\"lower-alpha\"><li id=\"li-50\"><p id=\"p-154\">$f: {\\mathbb R} \\rightarrow {\\mathbb R}$ defined by $f(x) = e^x$</p></li><li id=\"li-51\"><p id=\"p-155\">$f: {\\mathbb Z} \\rightarrow {\\mathbb Z}$ defined by $f(n) = n^2 + 3$</p></li><li id=\"li-52\"><p id=\"p-156\">$f: {\\mathbb R} \\rightarrow {\\mathbb R}$ defined by $f(x) = \\sin x$</p></li><li id=\"li-53\"><p id=\"p-157\">$f: {\\mathbb Z} \\rightarrow {\\mathbb Z}$ defined by $f(x) = x^2$</p></li></ol><div class=\"solutions\"><span class=\"solution\"><a knowl=\"\" class=\"id-ref\" refid=\"hk-hint-7\" id=\"hint-7\"><span class=\"type\">Hint</span></a></span><div id=\"hk-hint-7\" class=\"hidden-content tex2jax_ignore\"><span class=\"solution\"><p id=\"p-158\">(a) $f$ is one-to-one but not onto. $f({\\mathbb R} ) = \\{ x \\in {\\mathbb R} : x \\gt 0 \\}\\text{.}$  (c) $f$ is neither one-to-one nor onto.  $f(\\mathbb R) = \\{ x : -1 \\leq x \\leq 1 \\}\\text{.}$</p></span></div></div></article></div>"]},
{"cell_type":"markdown", "metadata":{}, "source":["<div class=\"mathbook-content\"><article class=\"exercise-like\" id=\"exercise-19\"><h6 class=\"heading\"><span class=\"codenumber\">19</span></h6><p id=\"p-159\">Let $f :A \\rightarrow B$ and $g : B \\rightarrow C$ be invertible mappings; that is, mappings such that $f^{-1}$ and $g^{-1}$ exist. Show that $(g \\circ f)^{-1} =f^{-1} \\circ g^{-1}\\text{.}$</p></article></div>"]},
{"cell_type":"markdown", "metadata":{}, "source":["<div class=\"mathbook-content\"><article class=\"exercise-like\" id=\"exercise-20\"><h6 class=\"heading\"><span class=\"codenumber\">20</span></h6><ol id=\"p-160\" class=\"lower-alpha\"><li id=\"li-54\"><p id=\"p-161\">Define a function $f: {\\mathbb N} \\rightarrow {\\mathbb N}$ that is one-to-one but not onto.</p></li><li id=\"li-55\"><p id=\"p-162\">Define a function $f: {\\mathbb N} \\rightarrow {\\mathbb N}$ that is onto but not one-to-one.</p></li></ol><div class=\"solutions\"><span class=\"solution\"><a knowl=\"\" class=\"id-ref\" refid=\"hk-hint-8\" id=\"hint-8\"><span class=\"type\">Hint</span></a></span><div id=\"hk-hint-8\" class=\"hidden-content tex2jax_ignore\"><span class=\"solution\"><p id=\"p-163\">(a) $f(n) = n + 1\\text{.}$</p></span></div></div></article></div>"]},
{"cell_type":"markdown", "metadata":{}, "source":["<div class=\"mathbook-content\"><article class=\"exercise-like\" id=\"exercise-21\"><h6 class=\"heading\"><span class=\"codenumber\">21</span></h6><p id=\"p-164\">Prove the relation defined on ${\\mathbb R}^2$ by $(x_1, y_1 ) \\sim (x_2, y_2)$ if $x_1^2 + y_1^2 = x_2^2 + y_2^2$ is  an equivalence relation.</p></article></div>"]},
{"cell_type":"markdown", "metadata":{}, "source":["<div class=\"mathbook-content\"><article class=\"exercise-like\" id=\"exercise-22\"><h6 class=\"heading\"><span class=\"codenumber\">22</span></h6><p id=\"p-165\">Let $f : A \\rightarrow B$ and $g : B \\rightarrow C$ be maps. </p><ol class=\"lower-alpha\"><li id=\"li-56\"><p id=\"p-166\">If $f$ and $g$ are both one-to-one functions, show that $g \\circ f$ is one-to-one.</p></li><li id=\"li-57\"><p id=\"p-167\">If $g \\circ f$ is onto, show that $g$ is onto.</p></li><li id=\"li-58\"><p id=\"p-168\">If $g \\circ f$ is one-to-one, show that $f$ is one-to-one.</p></li><li id=\"li-59\"><p id=\"p-169\">If $g \\circ f$ is one-to-one and $f$ is onto, show that $g$ is one-to-one.</p></li><li id=\"li-60\"><p id=\"p-170\">If $g \\circ f$ is onto and $g$ is one-to-one, show that $f$ is onto.</p></li></ol><div class=\"solutions\"><span class=\"solution\"><a knowl=\"\" class=\"id-ref\" refid=\"hk-hint-9\" id=\"hint-9\"><span class=\"type\">Hint</span></a></span><div id=\"hk-hint-9\" class=\"hidden-content tex2jax_ignore\"><span class=\"solution\"><p id=\"p-171\">(a) Let $x, y \\in A\\text{.}$ Then $g(f(x)) = (g \\circ f)(x) = (g \\circ f)(y) = g(f(y))\\text{.}$  Thus, $f(x) = f(y)$ and $x = y\\text{,}$  so $g \\circ f$ is one-to-one. (b) Let $c \\in C\\text{,}$ then $c = (g \\circ f)(x) = g(f(x))$ for some $x \\in A\\text{.}$ Since $f(x) \\in B\\text{,}$ $g$ is onto.</p></span></div></div></article></div>"]},
{"cell_type":"markdown", "metadata":{}, "source":["<div class=\"mathbook-content\"><article class=\"exercise-like\" id=\"exercise-23\"><h6 class=\"heading\"><span class=\"codenumber\">23</span></h6><p id=\"p-172\">Define a function on the real numbers by</p><div class=\"displaymath\">\n\\begin{equation*}\nf(x) = \\frac{x + 1}{x - 1}.\n\\end{equation*}\n</div><p>What are the domain and range of $f\\text{?}$ What is the inverse of $f\\text{?}$  Compute $f \\circ f^{-1}$ and $f^{-1} \\circ f\\text{.}$</p><div class=\"solutions\"><span class=\"solution\"><a knowl=\"\" class=\"id-ref\" refid=\"hk-hint-10\" id=\"hint-10\"><span class=\"type\">Hint</span></a></span><div id=\"hk-hint-10\" class=\"hidden-content tex2jax_ignore\"><span class=\"solution\"><p id=\"p-173\">$f^{-1}(x) = (x+1)/(x-1)\\text{.}$</p></span></div></div></article></div>"]},
{"cell_type":"markdown", "metadata":{}, "source":["<div class=\"mathbook-content\"><article class=\"exercise-like\" id=\"exercise-24\"><h6 class=\"heading\"><span class=\"codenumber\">24</span></h6><p id=\"p-174\">Let $f: X \\rightarrow Y$ be a map with $A_1, A_2 \\subset X$ and $B_1, B_2 \\subset Y\\text{.}$ </p><ol class=\"lower-alpha\"><li id=\"li-61\"><p id=\"p-175\">Prove $f( A_1 \\cup A_2 ) = f( A_1) \\cup f( A_2 )\\text{.}$</p></li><li id=\"li-62\"><p id=\"p-176\">Prove $f( A_1 \\cap A_2 ) \\subset f( A_1) \\cap f( A_2 )\\text{.}$  Give an example in which equality fails.</p></li><li id=\"li-63\"><p id=\"p-177\">Prove $f^{-1}( B_1 \\cup B_2 ) = f^{-1}( B_1) \\cup f^{-1}(B_2 )\\text{,}$ where</p><div class=\"displaymath\">\n\\begin{equation*}\nf^{-1}(B) = \\{ x \\in X : f(x) \\in B \\}.\n\\end{equation*}\n</div></li><li id=\"li-64\"><p id=\"p-178\">Prove $f^{-1}( B_1 \\cap B_2 ) = f^{-1}( B_1) \\cap f^{-1}( B_2 )\\text{.}$</p></li><li id=\"li-65\"><p id=\"p-179\">Prove $f^{-1}( Y \\setminus B_1 ) = X \\setminus f^{-1}( B_1)\\text{.}$</p></li></ol><div class=\"solutions\"><span class=\"solution\"><a knowl=\"\" class=\"id-ref\" refid=\"hk-hint-11\" id=\"hint-11\"><span class=\"type\">Hint</span></a></span><div id=\"hk-hint-11\" class=\"hidden-content tex2jax_ignore\"><span class=\"solution\"><p id=\"p-180\">(a) Let $y \\in f(A_1 \\cup A_2)\\text{.}$  Then there exists an $x \\in A_1 \\cup A_2$ such that $f(x) = y\\text{.}$  Hence, $y \\in f(A_1)$ or $f(A_2) \\text{.}$  Therefore, $y \\in f(A_1) \\cup f(A_2)\\text{.}$ Consequently, $f(A_1 \\cup A_2) \\subset f(A_1) \\cup f(A_2)\\text{.}$ Conversely, if $y \\in f(A_1) \\cup f(A_2)\\text{,}$ then $y \\in f(A_1)$ or $f(A_2)\\text{.}$  Hence, there exists an $x$ in $A_1$ or  $A_2$ such that $f(x) = y\\text{.}$  Thus, there exists an $x \\in A_1 \\cup A_2$ such that $f(x) = y\\text{.}$  Therefore, $f(A_1) \\cup f(A_2) \\subset f(A_1 \\cup A_2)\\text{,}$ and $f(A_1 \\cup A_2) = f(A_1) \\cup f(A_2)\\text{.}$</p></span></div></div></article></div>"]},
{"cell_type":"markdown", "metadata":{}, "source":["<div class=\"mathbook-content\"><article class=\"exercise-like\" id=\"exercise-25\"><h6 class=\"heading\"><span class=\"codenumber\">25</span></h6><p id=\"p-181\">Determine whether or not the following relations are equivalence relations on the given set.  If the relation is an equivalence relation, describe the partition given by it.  If the relation is not an equivalence relation, state why it fails to be one. </p><ol class=\"lower-alpha cols2\"><li id=\"li-66\"><p id=\"p-182\">$x \\sim y$ in ${\\mathbb R}$ if $x \\geq y$</p></li><li id=\"li-67\"><p id=\"p-183\">$m \\sim n$ in ${\\mathbb Z}$ if $mn > 0$</p></li><li id=\"li-68\"><p id=\"p-184\">$x \\sim y$ in ${\\mathbb R}$ if $|x - y| \\leq 4$</p></li><li id=\"li-69\"><p id=\"p-185\">$m \\sim n$ in ${\\mathbb Z}$ if $m \\equiv n \\pmod{6}$</p></li></ol><div class=\"solutions\"><span class=\"solution\"><a knowl=\"\" class=\"id-ref\" refid=\"hk-hint-12\" id=\"hint-12\"><span class=\"type\">Hint</span></a></span><div id=\"hk-hint-12\" class=\"hidden-content tex2jax_ignore\"><span class=\"solution\"><p id=\"p-186\">(a) The relation fails to be symmetric. (b) The relation is not reflexive, since 0 is not equivalent to itself. (c) The relation is not transitive.</p></span></div></div></article></div>"]},
{"cell_type":"markdown", "metadata":{}, "source":["<div class=\"mathbook-content\"><article class=\"exercise-like\" id=\"exercise-26\"><h6 class=\"heading\"><span class=\"codenumber\">26</span></h6><p id=\"p-187\">Define a relation $\\sim$ on ${\\mathbb R}^2$ by stating that $(a, b) \\sim (c, d)$ if and only if $a^2 + b^2 \\leq c^2 + d^2\\text{.}$ Show that $\\sim$ is reflexive and transitive but not symmetric.</p></article></div>"]},
{"cell_type":"markdown", "metadata":{}, "source":["<div class=\"mathbook-content\"><article class=\"exercise-like\" id=\"exercise-27\"><h6 class=\"heading\"><span class=\"codenumber\">27</span></h6><p id=\"p-188\">Show that an $m \\times n$ matrix gives rise to a well-defined  map from ${\\mathbb R}^n$ to ${\\mathbb R}^m\\text{.}$</p></article></div>"]},
{"cell_type":"markdown", "metadata":{}, "source":["<div class=\"mathbook-content\"><article class=\"exercise-like\" id=\"exercise-28\"><h6 class=\"heading\"><span class=\"codenumber\">28</span></h6><p id=\"p-189\">Find the error in the following argument by providing a counterexample. “The reflexive property is redundant in the axioms for an equivalence relation.  If $x \\sim y\\text{,}$ then $y \\sim x$ by the symmetric property.  Using the transitive property, we can deduce that $x \\sim x\\text{.}$”</p><div class=\"solutions\"><span class=\"solution\"><a knowl=\"\" class=\"id-ref\" refid=\"hk-hint-13\" id=\"hint-13\"><span class=\"type\">Hint</span></a></span><div id=\"hk-hint-13\" class=\"hidden-content tex2jax_ignore\"><span class=\"solution\"><p id=\"p-190\">Let $X = {\\mathbb N} \\cup \\{ \\sqrt{2}\\, \\}$ and define $x \\sim y$ if $x + y \\in {\\mathbb N}\\text{.}$</p></span></div></div></article></div>"]},
{"cell_type":"markdown", "metadata":{}, "source":["<div class=\"mathbook-content\"><article class=\"exercise-like\" id=\"exercise-29\"><h6 class=\"heading\"><span class=\"codenumber\">29</span><span class=\"title\">Projective Real Line</span></h6><p id=\"p-191\">Define a relation on ${\\mathbb R}^2 \\setminus  \\{ (0,0) \\}$ by letting $(x_1, y_1) \\sim (x_2, y_2)$ if there exists a nonzero real number $\\lambda$ such that $(x_1, y_1)  = ( \\lambda x_2, \\lambda y_2)\\text{.}$  Prove that $\\sim$ defines an equivalence relation on ${\\mathbb R}^2 \\setminus (0,0)\\text{.}$  What are the corresponding  equivalence classes?  This equivalence relation defines the projective line, denoted by  ${\\mathbb P}({\\mathbb R}) \\text{,}$ which is very important in geometry.</p></article></div>"]}
],
"nbformat": 4, "nbformat_minor": 0, "metadata": {"kernelspec": {"display_name": "", "name": "sagemath"}, "language_info": {"codemirror_mode": {"name": "ipython", "version": 2}, "file_extension": ".py", "mimetype": "text/x-python", "name": "python", "nbconvert_exporter": "python", "pygments_lexer": "ipython2", "version": "2.7.8"}, "name": "exercises-sets.ipynb"}
}